Tactic Refined. central_step added as bottom level, with autounfold provided. The HintDb for Ranko has the name "magic_book".

Babel/Morrise86.v
@@ -1,6 +1,9 @@
 Require Import POrder POrderSet TerminalDogma.premises
                                 TerminalDogma.Extensionality.
-Require Import SetFacility POrderFacility.
+
+Require Import SetFacility 
+                POrderFacility 
+                POrderBool.
 
 Require Import Ranko.
 
@@ -9,11 +12,46 @@ Unset Strict Implicit.
 Unset Printing Implicit Defensive.
 
 
+
+
 (** The type of state. *)
 Axiom Stt : Type.
 
 
-Definition Sta := 𝒫(Stt).
+(** >>> *)
+Import LeibnizEqOrder.CanonicalStruct.
 
+Definition Sta := [poset of Stt].
+
+
+
+(** >>> *)
+Import FunPointwiseOrder.CanonicalStruct.
+Import BoolOrder.CanonicalStruct.
+
+Definition Asn := [clattice of [Sta ↦ᵐ bool]].
+
+
+
+(** some wrapping definitions *)
+Definition asn_impl_comp (P Q : Asn) : Sta -> bool := fun s => (P s ==> Q s).
+Notation "P ⇒ Q" := (asn_impl_comp P Q) (at level 40).
+
+Definition uni_quantification (P : Asn) : Prop := forall s, P s.
+Notation "⌈ P ⌉" := (uni_quantification P).
+
+
+#[local] Hint Unfold asn_impl_comp : magic_book.
+#[local] Hint Unfold uni_quantification : magic_book.
+
+Lemma Lemma_3_1 (P Q : Asn) :
+    P ⊑ Q <-> ⌈ P ⇒ Q ⌉.
+Proof.
+    ranko.
+
+    apply /implyP. by apply (H s).
+
+    by move : (implyP (H x) H0).
+Qed.
 
 
